Rename Framing modules into regular Steel modules

pulse/ulib/experimental/Steel.HigherReference.fst
@@ -23,7 +23,7 @@ open FStar.Real
 open FStar.PCM
 open Steel.FractionalPermission
 module Atomic = Steel.Effect.Atomic
-module SB = Steel.SteelT.Basics
+//module SB = Steel.SteelT.Basics
 
 let fractional (a:Type u#1) = option (a & perm)
 #push-options "--query_stats"
@@ -125,13 +125,13 @@ let comm (#opened_invariants:inames)
   : SteelAtomic unit opened_invariants unobservable
                 (p `star` q)
                 (fun x -> q `star` p)
-  = Atomic.change_slprop _ _ (fun m -> Mem.star_commutative p q)
+  = Atomic.change_slprop (p `star` q) (q `star` p) (fun m -> Mem.star_commutative p q)
 
 let intro_perm_ok #uses (p:perm{perm_ok p}) (q:slprop)
   : SteelAtomic unit uses unobservable
                 q
                 (fun _ -> q `star` pure (perm_ok p))
-  = Atomic.change_slprop _ _
+  = Atomic.change_slprop q (q `star` pure (perm_ok p))
     (fun m -> emp_unit q; pure_star_interp q (perm_ok p) m)
 
 let elim_perm_ok #uses (p:perm)
@@ -139,7 +139,7 @@ let elim_perm_ok #uses (p:perm)
                 (pure (perm_ok p))
                 (fun _ -> emp)
   = let _ = Atomic.elim_pure (perm_ok p) in
-    Atomic.return_atomic p
+    p
 
 let intro_pts_to (p:perm{perm_ok p}) #a #uses (#v:erased a) (r:ref a) (_:unit)
   : SteelAtomic unit uses unobservable
@@ -147,71 +147,78 @@ let intro_pts_to (p:perm{perm_ok p}) #a #uses (#v:erased a) (r:ref a) (_:unit)
                 (fun _ -> pts_to r p v)
   = intro_perm_ok p _
 
-let intro_pure (#a:_) (#p:a -> slprop) (q:perm { perm_ok q }) (x:a)
-  : SteelT a (p x) (fun y -> p y `star` pure (perm_ok q))
-  = intro_perm_ok q _;
-    SB.return x
-
-let drop_l_atomic #uses (#p #q:slprop)  ()
+let drop_l_atomic #uses (p q:slprop)  ()
   : SteelAtomic unit uses unobservable (p `star` q) (fun _ -> q)
-  = Atomic.change_slprop _ _ (affine_star p q)
+  = Atomic.change_slprop (p `star` q) q (affine_star p q)
 
 let elim_pure_atomic #uses  (#p:perm -> slprop) (q:perm)
   : SteelAtomic (q':perm{perm_ok q' /\ q == q'}) uses unobservable
                 (p q `star` pure (perm_ok q))
                 (fun q' -> p q')
-  = comm();
-    let q' = Atomic.frame _ (fun _ -> elim_perm_ok q) in
-    h_assert_atomic (emp `star` p q);
-    drop_l_atomic ();
-    Atomic.return_atomic q'
-
-let elim_perm_ok_star (#p:slprop) (q:perm)
-  : SteelT (_:unit{perm_ok q}) (p `star` pure (perm_ok q))
-           (fun _ -> p)
-  = let _ = elim_pure_atomic #Set.empty #(fun _ -> p) q in
-    SB.return ()
+  = let (q':perm {perm_ok q' /\ q == q'}) = elim_perm_ok q in
+    Atomic.change_slprop (p q) (p q') (fun _ -> ());
+    q'
 
 let alloc #a x =
   let v = Some (x, full_perm) in
   assert (FStar.PCM.composable pcm_frac v None);
   assert (compatible pcm_frac v v);
-  let x = Steel.Effect.alloc v in
-  intro_pure full_perm x
+  let r = Steel.Effect.alloc v in
+  Steel.Effect.change_slprop (Steel.Memory.pts_to r v) (pts_to r full_perm (hide x))
+    (fun m -> emp_unit (pts_to_raw r full_perm x); pure_star_interp (pts_to_raw r full_perm x) (perm_ok full_perm) m);
+  r
 
 let read (#a:Type) (#p:perm) (#v:erased a) (r:ref a)
   = let v1 : erased (fractional a) = Ghost.hide (Some (Ghost.reveal v, p)) in
-    elim_perm_ok_star p;
+    Steel.Effect.change_slprop (pts_to r p v) (Mem.pts_to r v1 `star` pure (perm_ok p)) (fun _ -> ());
+    let _ = elim_perm_ok p in
     let v2 = Steel.Effect.read r v1 in
+    Steel.Effect.change_slprop (Steel.Memory.pts_to r v1) (pts_to r p v)
+        (fun m -> emp_unit (pts_to_raw r p v); pure_star_interp (pts_to_raw r p v) (perm_ok p) m);
     assert (compatible pcm_frac v1 v2);
     let Some (x, _) = v2 in
-    intro_pure p x
+    Steel.Effect.change_slprop (pts_to r p v) (pts_to r p x) (fun _ -> ());
+    x
+
+assume
+val witness_h_exists (#a:Type) (p:(a -> slprop){is_frame_monotonic p}) (_:unit)
+  : SteelT (Ghost.erased a) (h_exists p) (fun x -> p x)
 
 let read_refine (#a:Type) (#p:perm) (q:a -> slprop) (r:ref a)
   : SteelT a (h_exists (fun (v:a) -> pts_to r p v `star` q v))
-             (fun (v:a) -> pts_to r p v `star` q v)
+                (fun v -> pts_to r p v `star` q v)
   = pts_to_witinv r p;
     star_is_witinv_left (fun (v:a) -> pts_to r p v) q;
-    let vs = SB.witness_h_exists () in
-    SB.h_assert (pts_to r p vs `star` q vs);
-    let v = SB.frame (fun _ -> read #a #p #vs r) _ in
-    SB.h_assert (pts_to r p v `star` q v);
-    SB.return v
+    let vs:erased a = witness_h_exists (fun (v:a) -> pts_to r p v `star` q v) () in
+
+    Steel.Effect.change_slprop (pts_to r p (Ghost.hide (Ghost.reveal vs)) `star` q vs) (pts_to r p vs `star` q vs) (fun _ -> ());
+
+    let v = read #a #p #vs r in
+
+    Steel.Effect.change_slprop (pts_to r p v `star` q vs) (pts_to r p v `star` q v) (fun _ -> ());
+    v
 
 let write (#a:Type) (#v:erased a) (r:ref a) (x:a)
   : SteelT unit (pts_to r full_perm v) (fun _ -> pts_to r full_perm x)
   = let v_old : erased (fractional a) = Ghost.hide (Some (Ghost.reveal v, full_perm)) in
     let v_new : fractional a = Some (x, full_perm) in
-    elim_perm_ok_star full_perm;
+    Steel.Effect.change_slprop (pts_to r full_perm v) (Mem.pts_to r v_old `star` pure (perm_ok full_perm)) (fun _ -> ());
+
+    let _ = elim_perm_ok full_perm in
     Steel.Effect.write r v_old v_new;
-    intro_pure full_perm ()
+    Steel.Effect.change_slprop (Mem.pts_to r v_new) (pts_to r full_perm x)
+        (fun m -> emp_unit (pts_to_raw r full_perm x); pure_star_interp (pts_to_raw r full_perm x) (perm_ok full_perm) m)
 
 let free (#a:Type) (#v:erased a) (r:ref a)
   : SteelT unit (pts_to r full_perm v) (fun _ -> emp)
   = let v_old : erased (fractional a) = Ghost.hide (Some (Ghost.reveal v, full_perm)) in
-    elim_perm_ok_star full_perm;
+    Steel.Effect.change_slprop
+      (pts_to r full_perm v)
+      (Mem.pts_to r v_old `star` pure (perm_ok full_perm))
+      (fun _ -> ());
+    let _ = elim_perm_ok full_perm in
     Steel.Effect.free r v_old;
-    drop _
+    drop (Mem.pts_to r (Mkpcm'?.one (Mkpcm?.p pcm_frac)))
 
 (* move these to Mem *)
 let mem_share_atomic_raw (#a:Type) (#uses:_) (#p:perm{perm_ok p}) (r:ref a)
@@ -231,19 +238,15 @@ let share_atomic (#a:Type) #uses (#p:perm) (#v:erased a) (r:ref a)
   : SteelAtomic unit uses unobservable
                (pts_to r p v)
                (fun _ -> pts_to r (half_perm p) v `star` pts_to r (half_perm p) v)
-  = let p = elim_pure_atomic #_ #(fun q -> pts_to_raw r q v) p in
-    share_atomic_raw r v;
-    h_assert_atomic (pts_to_raw r (half_perm p) v `star` pts_to_raw r (half_perm p) v);
-    Steel.Effect.Atomic.frame _
-                                  (intro_pts_to (half_perm p) r);
-    h_assert_atomic (pts_to r (half_perm p) v `star` pts_to_raw r (half_perm p) v);
-    comm ();
-    h_assert_atomic (pts_to_raw r (half_perm p) v `star` pts_to r (half_perm p) v);
-    Steel.Effect.Atomic.frame #unit #uses #unobservable
-                                  #(pts_to_raw r (half_perm p) v)
-                                  #(fun _ -> pts_to r (half_perm p) v)
-                                  (pts_to r (half_perm p) v)
-                                  (intro_pts_to (half_perm p) r)
+  = let v_old : erased (fractional a) = Ghost.hide (Some (Ghost.reveal v, p)) in
+    Atomic.change_slprop
+      (pts_to r p v)
+      (pts_to_raw r p v `star` pure (perm_ok p))
+      (fun _ -> ());
+    let _ = Atomic.elim_pure (perm_ok p) in
+    share_atomic_raw #_ #_ #p r v;
+    intro_pts_to (half_perm p) r ();
+    intro_pts_to (half_perm p) r ()
 
 let share r = share_atomic r
 
@@ -262,12 +265,19 @@ let gather_atomic_raw (#a:Type) (#uses:_) (#p0 #p1:perm) (r:ref a) (v0:erased a)
   = as_atomic_action (mem_gather_atomic_raw r v0 v1)
 
 let gather_atomic (#a:Type) (#uses:_) (#p0:perm) (#p1:perm) (#v0 #v1:erased a) (r:ref a)
-  = let p0 = Steel.Effect.Atomic.frame _ (fun _ -> elim_pure_atomic p0) in
-    comm();
-    let p1 = Steel.Effect.Atomic.frame _ (fun _ -> elim_pure_atomic p1) in
-    comm();
-    h_assert_atomic (pts_to_raw r p0 v0 `star` pts_to_raw r p1 v1);
-    let _ = gather_atomic_raw r v0 v1 in
+  = let v0_old : erased (fractional a) = Ghost.hide (Some (Ghost.reveal v0, p0)) in
+    let v1_old : erased (fractional a) = Ghost.hide (Some (Ghost.reveal v1, p1)) in
+    Atomic.change_slprop
+      (pts_to r p0 v0)
+      (pts_to_raw r p0 v0 `star` pure (perm_ok p0))
+      (fun _ -> ());
+    Atomic.change_slprop
+      (pts_to r p1 v1)
+      (pts_to_raw r p1 v1 `star` pure (perm_ok p1))
+      (fun _ -> ());
+    let _ = Atomic.elim_pure (perm_ok p0) in
+    let _ = Atomic.elim_pure (perm_ok p1) in
+    let _ = gather_atomic_raw #_ #_ #p0 #p1 r v0 v1 in
     intro_pts_to (sum_perm p0 p1) r ()
 
 let gather r = gather_atomic r
